theories/Logic/ProgramLogic.v
@@ -1,0 +1,304 @@
+From Metaprog Require Import Prelude.
+From Metaprog Require Export Control.Meta MetaTheory.EvarMap Logic.Lattice.
+
+(** This module defines the program logic. *)
+
+(** [gstate] is the ghost state we use when verifying meta-programs
+    using the program logic. *)
+Definition gstate : Type := evar_map.
+
+(***********************************************************************)
+(** * Logical effect handlers. *)
+(***********************************************************************)
+
+(** A logical effect handler for effect [E] is a predicate
+    transformer on events [e : E A], i.e. a function which maps postconditions
+    [Φ : A -> gstate -> Prop] to preconditions [h e Φ : gstate -> Prop].
+
+    Effect handlers are additionally required to be monotonic w.r.t. [Φ]
+    i.e. to obey the consequence rule. *)
+Record handler (E : Type -> Type) := mkhandler {
+  (** The actual function of the handler. *)
+  handler_fun A : E A -> (A -> gstate -> Prop) -> (gstate -> Prop) ;
+  (** A proof of monotonicity. *)
+  handler_mono A (e : E A) Φ Φ' g :
+    (forall x g, Φ x g -> Φ' x g) ->
+    handler_fun _ e Φ g ->
+    handler_fun _ e Φ' g
+}.
+
+Arguments mkhandler {E}.
+Arguments handler_fun {E} : simpl nomatch.
+Arguments handler_mono {E}.
+
+Coercion handler_fun : handler >-> Funclass.
+
+(** We can freely change the postcondition of a handler to
+    an equivalent one. *)
+Lemma handler_equiv {E A} (h : handler E) (e : E A) Φ Φ' g :
+  (forall x g, Φ x g <-> Φ' x g) ->
+  h _ e Φ g <-> h _ e Φ' g.
+Proof.
+intros H. split ; intros H'.
+- eapply handler_mono ; [|exact H']. firstorder.
+- eapply handler_mono ; [|exact H']. firstorder.
+Qed.
+
+(** Handlers form a complete lattice. *)
+Program Instance CompleteLattice_handler {E} : CompleteLattice (handler E) := {|
+  leq h h' := leq (handler_fun h) (handler_fun h') ;
+  weq h h' := weq (handler_fun h) (handler_fun h') ;
+  isup I P f := {| handler_fun := isup P (fun i => handler_fun (f i)) |} ;
+  iinf I P f := {| handler_fun := iinf P (fun i => handler_fun (f i)) |} ;
+  cup h h' := {| handler_fun := cup (handler_fun h) (handler_fun h') |} ;
+  cap h h' := {| handler_fun := cap (handler_fun h) (handler_fun h') |} ;
+  bot := {| handler_fun := bot |} ;
+  top := {| handler_fun := top |} ;
+|}.
+Next Obligation. intros. cbn in *. destruct H0. eexists ; eauto using handler_mono. Qed.
+Next Obligation. intros. cbn in *. eauto using handler_mono. Qed.
+Next Obligation. intros. cbn in *. destruct H0 ; [left | right] ; eauto using handler_mono. Qed.
+Next Obligation. intros. cbn in *. destruct H0 ; split ; eauto using handler_mono. Qed.
+Next Obligation. intros. cbn in *. firstorder. Qed.
+Next Obligation. intros. cbn in *. firstorder. Qed.
+Next Obligation.
+intros E. split.
+- intros h. reflexivity.
+- intros h1 h2 h3 H1 H2. now transitivity h2.
+Qed.
+Next Obligation. intros E h h'. apply weq_spec. Qed.
+Next Obligation. intros E I is hs h. apply leq_isup_x. Qed.
+Next Obligation. intros E I is hs h. apply leq_x_iinf. Qed.
+Next Obligation. intros E h1 h2 h3. apply leq_cup_x. Qed.
+Next Obligation. intros E h1 h2 h3. apply leq_x_cap. Qed.
+Next Obligation. intros E h. apply leq_x_top. Qed.
+Next Obligation. intros E h. apply leq_bot_x. Qed.
+
+(***********************************************************************)
+(** * Sum of handlers. *)
+(***********************************************************************)
+
+(** [handler_sum h h'] is the disjoint sum of handlers [h] and [h']. *)
+Program Definition handler_sum {E E'} (h : handler E) (h' : handler E') :
+  handler (E +' E') :=
+  {| handler_fun := fun A (e : (E +' E') A) =>
+    match e with
+    | sumE_l e => h _ e
+    | sumE_r e => h' _ e
+    end
+  |}.
+Next Obligation. destruct e ; eapply handler_mono ; eassumption. Qed.
+
+(*Lemma handler_sum_mono {E1 E E'} (hh : handler E1 -> handler E S) (hh' : handler E1 S1 -> handler E' S) :
+  monotone hh ->
+  monotone hh' ->
+  monotone (fun h => handler_sum (hh h) (hh' h)).
+Proof.
+intros H1 H2 h h' Hh. cbn in *. intros A [e | e] Φ s ; cbn.
+- now apply H1.
+- now apply H2.
+Qed.*)
+
+(***********************************************************************)
+(** * Sub-handlers. *)
+(***********************************************************************)
+
+(** A handler [h : handler E] is a sub-handler of [h' : handler E'] iff:
+    - [E] is included in [E'].
+    - [h] and [h'] agree on every event [e : E].
+
+    Typically, [h] and [h'] are subhandlers of [handler_sum h h'].
+*)
+Class subhandler {E E'} `{E -< E'} (h : handler E) (h' : handler E') := {
+  handle_inj {A} (e : E A) (Φ : A -> gstate -> Prop) g :
+    h' _ (inj_event e) Φ g <-> h _ e Φ g
+}.
+
+#[export] Instance subhandler_refl {E} (h : handler E) :
+  subhandler h h.
+Proof. constructor. reflexivity. Qed.
+
+#[export] Instance subhandler_sum_l {E E1 E2 }
+  (h : handler E) (h1 : handler E1) (h2 : handler E2) `{subhandler _ _ h h1} :
+  subhandler h (handler_sum h1 h2).
+Proof.
+constructor. intros A e Φ g. cbn. rewrite handle_inj. reflexivity.
+Qed.
+
+#[export] Instance subhandler_sum_r {E E1 E2}
+  (h : handler E) (h1 : handler E1) (h2 : handler E2) `{subhandler _ _ h h2} :
+  subhandler h (handler_sum h1 h2).
+Proof.
+constructor. intros A e Φ g. cbn. rewrite handle_inj. reflexivity.
+Qed.
+
+(**************************************************************************)
+(** *** Weakest-precondition. *)
+(**************************************************************************)
+
+Section WeakestPrecondition.
+  Context {E : Type -> Type} (hE : handler E).
+
+  (** Weakest-precondition functor. *)
+  Program Definition wp_step (R : handler (meta E)) : handler (meta E) := {|
+    handler_fun _ m :=
+      match m with
+      | Ret x => fun Φ g => Φ x g
+      | Bind m k => fun Φ g => R _ m (fun x g' => R _ (k x) Φ g') g
+      | Vis e => fun Φ g => hE _ e Φ g
+      end
+  |}.
+  Next Obligation.
+  intros R A m Φ Φ' g HΦ. destruct m.
+  - firstorder.
+  - apply handler_mono. intros x g'. apply handler_mono. firstorder.
+  - apply handler_mono. firstorder.
+  Qed.
+
+  Lemma wp_step_mono : monotone wp_step.
+  Proof.
+  intros R R' HR A m Φ g. cbn. destruct m ; cbn.
+  - firstorder.
+  - intros H. cut (R _ m (fun x g' => R' _ (m0 x) Φ g') g).
+    + apply HR.
+    + revert H. apply handler_mono. intros x g'. apply HR.
+  - firstorder.
+  Qed.
+
+  (** The weakest-precondition [wp] is constructed by taking the
+      least fixpoint of [wp_step]. *)
+  Definition wp : handler (meta E) := lfp wp_step.
+
+  (** Consequence rule. *)
+  Lemma wp_consequence {A} {m : meta E A} {Φ Φ' g} :
+    (forall x g, Φ x g -> Φ' x g) ->
+    wp _ m Φ g ->
+    wp _ m Φ' g.
+  Proof. apply handler_mono. Qed.
+
+  Lemma wp_equiv {A} (m : meta E A) {Φ Φ' g} :
+    (forall x g, Φ x g <-> Φ' x g) ->
+    wp _ m Φ g <-> wp _ m Φ' g.
+  Proof. apply handler_equiv. Qed.
+
+  Lemma wp_unfold {A} {m : meta E A} {Φ g} :
+    wp _ m Φ g <-> wp_step wp _ m Φ g.
+  Proof.
+  pose proof (H := lfp_fixpoint wp_step wp_step_mono).
+  specialize (H A m Φ g). cbn in H. rewrite H. reflexivity.
+  Qed.
+
+  Lemma wp_Ret {A} {x : A} {Φ g} :
+    wp _ (Ret x) Φ g <-> Φ x g.
+  Proof. rewrite wp_unfold. reflexivity. Qed.
+
+  Lemma wp_Bind {A B} {m : meta E A} {f : A -> meta E B} {Φ g} :
+    wp _ (Bind m f) Φ g <-> wp _ m (fun x g' => wp _ (f x) Φ g') g.
+  Proof. rewrite wp_unfold. reflexivity. Qed.
+
+  Lemma wp_Vis {A} {e : E A} {Φ g} :
+    wp _ (Vis e) Φ g <-> hE _ e Φ g.
+  Proof. rewrite wp_unfold. reflexivity. Qed.
+
+  (** Induction principle on [wp]. This relies on the fact that [wp] is defined
+      as a _least_ fixpoint instead of a greatest fixpoint. *)
+  Lemma wp_ind (R : handler (meta E)) :
+    (forall A a Φ g, Φ a g -> R A (Ret a) Φ g) ->
+    (forall A B m k Φ g, R A m (fun x g' => R B (k x) Φ g') g -> R B (Bind m k) Φ g) ->
+    (forall A e Φ g, hE A e Φ g -> R A (Vis e) Φ g) ->
+    forall A m Φ g, wp A m Φ g -> R A m Φ g.
+  Proof.
+  intros Hret Hbind Hvis. apply (lfp_smallest wp_step wp_step_mono).
+  cbn. intros A [a | m k | e] Φ g ; cbn.
+  - apply Hret.
+  - apply Hbind.
+  - apply Hvis.
+  Qed.
+
+  (** We might wonder what happens if we define [wp] as a _greatest_
+      fixpoint instead of a least fixpoint. Do we obtain a partial program logic?
+      Remarkably, we obtain the same program logic: to control whether the logic
+      is total/partial, we instead need to define the effect handler [hE] as
+      a least/greatest fixpoint. *)
+
+  (** Same as [wp] but as a _greatest_ fixpoint. *)
+  Definition wp' : handler (meta E) := gfp wp_step.
+
+  Lemma wp_unfold' {A} {m : meta E A} {Φ g} :
+    wp' _ m Φ g <-> wp_step wp' _ m Φ g.
+  Proof.
+  pose proof (H := gfp_fixpoint wp_step wp_step_mono).
+  specialize (H A m Φ g). cbn in H. rewrite H. reflexivity.
+  Qed.
+
+  (** The key property is that [wp'] admits the same induction (not coinduction)
+      principle as [wp]. *)
+  Lemma wp_ind' (R : handler (meta E)) :
+    (forall A a Φ g, Φ a g -> R A (Ret a) Φ g) ->
+    (forall A B m k Φ g, R A m (fun x g' => R B (k x) Φ g') g -> R B (Bind m k) Φ g) ->
+    (forall A e Φ g, hE A e Φ g -> R A (Vis e) Φ g) ->
+    forall A m Φ g, wp' A m Φ g -> R A m Φ g.
+  Proof.
+  intros Hret Hbind Hvis A m. induction m ; intros Φ g.
+  - rewrite wp_unfold'. cbn. apply Hret.
+  - rewrite wp_unfold'. cbn. intros H'. apply Hbind. apply IHm in H'. revert H'.
+    apply handler_mono. intros x g'. apply H.
+  - rewrite wp_unfold'. cbn. apply Hvis.
+  Qed.
+
+  Lemma wp_same_1 {A} (m : meta E A) Φ g :
+    wp _ m Φ g -> wp' _ m Φ g.
+  Proof.
+  revert A m Φ g. apply wp_ind.
+  - intros A a Φ g H. rewrite wp_unfold'. cbn. assumption.
+  - intros A B m k Φ g H. rewrite wp_unfold'. cbn. assumption.
+  - intros A e Φ g H. rewrite wp_unfold'. cbn. assumption.
+  Qed.
+
+  Lemma wp_same_2 {A} (m : meta E A) Φ g :
+    wp' _ m Φ g -> wp _ m Φ g.
+  Proof.
+  revert A m Φ g. apply wp_ind'.
+  - intros A a Φ g H. rewrite wp_Ret. assumption.
+  - intros A B m k Φ g H. rewrite wp_Bind. assumption.
+  - intros A e Φ g H. rewrite wp_Vis. assumption.
+  Qed.
+
+  (** This theorem justifies why we only use [wp] in the following,
+      both when constructing a total and a partial program logic. *)
+  Theorem wp_same {A} (m : meta E A) Φ g :
+    wp _ m Φ g <-> wp' _ m Φ g.
+  Proof. split ; [apply wp_same_1 | apply wp_same_2]. Qed.
+
+  (** As a consequence of [wp_same] we get a coinduction (i.e. introduction)
+      principle for [wp]. We could probably also show this from first principles
+      without using [wp_same]. *)
+  Lemma wp_coind (R : handler (meta E)) :
+    (forall A a Φ g, R A (Ret a) Φ g -> Φ a g) ->
+    (forall A B m k Φ g, R B (Bind m k) Φ g -> R A m (fun x g' => R B (k x) Φ g') g) ->
+    (forall A e Φ g, R A (Vis e) Φ g -> hE A e Φ g) ->
+    forall A m Φ g, R A m Φ g -> wp A m Φ g.
+  Proof.
+  intros Hret Hbind Hvis. setoid_rewrite wp_same. apply (gfp_greatest wp_step wp_step_mono).
+  cbn. intros A [a | m k | e] Φ g ; cbn.
+  - apply Hret.
+  - apply Hbind.
+  - apply Hvis.
+  Qed.
+
+End WeakestPrecondition.
+
+(* TODO: maybe use a better form of sealing. *)
+Arguments wp : simpl never.
+
+(** [wp] is a monotone functon from effect handlers to effect handlers. *)
+Lemma wp_mono {E} : monotone (@wp E).
+Proof.
+intros h h' Hh. cbn in *. intros A m Φ g.
+induction m in Φ, g |- *.
+- rewrite !wp_Ret. firstorder.
+- rewrite !wp_Bind. intros H1. cut (wp h _ m (fun x g' => wp h' _ (m0 x) Φ g') g).
+  + apply IHm.
+  + revert H1. apply wp_consequence. intros x g'. apply H.
+- rewrite !wp_Vis. apply Hh.
+Qed.
